more work on connection to Coq model

sail-riscv/RV64.v
@@ -158,11 +158,29 @@ Lemma regstate_eta (regs : regstate) :
   |}.
 Proof. now destruct regs. Qed.
 
+Lemma x2_nextPC regs n:
+  (x2 {[ regs with nextPC := n ]} ) = x2 regs.
+Proof. now rewrite (regstate_eta regs). Qed.
 Lemma x10_nextPC regs n:
   (x10 {[ regs with nextPC := n ]} ) = x10 regs.
 Proof. now rewrite (regstate_eta regs). Qed.
+Lemma nextPC_x10 regs n:
+  (nextPC {[ regs with x10 := n ]} ) = nextPC regs.
+Proof. now rewrite (regstate_eta regs). Qed.
 Lemma x11_nextPC regs n:
   (x11 {[ regs with nextPC := n ]} ) = x11 regs.
+Proof. now rewrite (regstate_eta regs). Qed.
+Lemma nextPC_x11 regs n:
+  (nextPC {[ regs with x11 := n ]} ) = nextPC regs.
+Proof. now rewrite (regstate_eta regs). Qed.
+Lemma mstatus_nextPC regs n:
+  (mstatus {[ regs with nextPC := n ]} ) = mstatus regs.
+Proof. now rewrite (regstate_eta regs). Qed.
+Lemma misa_nextPC regs n:
+  (misa {[ regs with nextPC := n ]} ) = misa regs.
+Proof. now rewrite (regstate_eta regs). Qed.
+Lemma cur_privilege_nextPC regs n:
+  (cur_privilege {[ regs with nextPC := n ]} ) = cur_privilege regs.
 Proof. now rewrite (regstate_eta regs). Qed.
 Lemma PC_nextPC regs n:
   (PC {[ regs with nextPC := n ]} ) = PC regs.
@@ -184,6 +202,10 @@ Lemma get_word_to_word n H (w : Word.word (Z.to_nat n)):
   get_word (to_word H w) = w.
 Proof. destruct n => //. Qed.
 
+Lemma get_word_inj n (m1 m2 : mword n):
+  get_word m1 = get_word m2 → m1 = m2.
+Proof. by destruct n. Qed.
+
 Lemma lt_Npow2 n n1:
   (0 ≤ n1)%Z →
   (n < NatLib.Npow2 (Z.to_nat n1))%N ↔ (Z.of_N n < 2 ^ n1)%Z.
@@ -192,7 +214,182 @@ Proof.
   rewrite -Npow2_pow Z_nat_N. etrans; [ apply N2Z.inj_lt |].
   by rewrite N2Z.inj_pow Z2N.id.
 Qed.
+(*
+Definition get_regval' (reg_name : string) (s : regstate) : option register_value :=
+  match reg_name with
+  | "satp" => Some (satp_ref.(regval_of) (satp_ref.(read_from) s))
+  | "tlb48" => Some (tlb48_ref.(regval_of) (tlb48_ref.(read_from) s))
+  | "tlb39" => Some (tlb39_ref.(regval_of) (tlb39_ref.(read_from) s))
+  | "htif_payload_writes" => Some (htif_payload_writes_ref.(regval_of) (htif_payload_writes_ref.(read_from) s))
+  | "htif_cmd_write" => Some (htif_cmd_write_ref.(regval_of) (htif_cmd_write_ref.(read_from) s))
+  | "htif_exit_code" => Some (htif_exit_code_ref.(regval_of) (htif_exit_code_ref.(read_from) s))
+  | "htif_done" => Some (htif_done_ref.(regval_of) (htif_done_ref.(read_from) s))
+  | "htif_tohost" => Some (htif_tohost_ref.(regval_of) (htif_tohost_ref.(read_from) s))
+  | "mtimecmp" => Some (mtimecmp_ref.(regval_of) (mtimecmp_ref.(read_from) s))
+  | "fcsr" => Some (fcsr_ref.(regval_of) (fcsr_ref.(read_from) s))
+  | "f31" => Some (f31_ref.(regval_of) (f31_ref.(read_from) s))
+  | "f30" => Some (f30_ref.(regval_of) (f30_ref.(read_from) s))
+  | "f29" => Some (f29_ref.(regval_of) (f29_ref.(read_from) s))
+  | "f28" => Some (f28_ref.(regval_of) (f28_ref.(read_from) s))
+  | "f27" => Some (f27_ref.(regval_of) (f27_ref.(read_from) s))
+  | "f26" => Some (f26_ref.(regval_of) (f26_ref.(read_from) s))
+  | "f25" => Some (f25_ref.(regval_of) (f25_ref.(read_from) s))
+  | "f24" => Some (f24_ref.(regval_of) (f24_ref.(read_from) s))
+  | "f23" => Some (f23_ref.(regval_of) (f23_ref.(read_from) s))
+  | "f22" => Some (f22_ref.(regval_of) (f22_ref.(read_from) s))
+  | "f21" => Some (f21_ref.(regval_of) (f21_ref.(read_from) s))
+  | "f20" => Some (f20_ref.(regval_of) (f20_ref.(read_from) s))
+  | "f19" => Some (f19_ref.(regval_of) (f19_ref.(read_from) s))
+  | "f18" => Some (f18_ref.(regval_of) (f18_ref.(read_from) s))
+  | "f17" => Some (f17_ref.(regval_of) (f17_ref.(read_from) s))
+  | "f16" => Some (f16_ref.(regval_of) (f16_ref.(read_from) s))
+  | "f15" => Some (f15_ref.(regval_of) (f15_ref.(read_from) s))
+  | "f14" => Some (f14_ref.(regval_of) (f14_ref.(read_from) s))
+  | "f13" => Some (f13_ref.(regval_of) (f13_ref.(read_from) s))
+  | "f12" => Some (f12_ref.(regval_of) (f12_ref.(read_from) s))
+  | "f11" => Some (f11_ref.(regval_of) (f11_ref.(read_from) s))
+  | "f10" => Some (f10_ref.(regval_of) (f10_ref.(read_from) s))
+  | "f9" => Some (f9_ref.(regval_of) (f9_ref.(read_from) s))
+  | "f8" => Some (f8_ref.(regval_of) (f8_ref.(read_from) s))
+  | "f7" => Some (f7_ref.(regval_of) (f7_ref.(read_from) s))
+  | "f6" => Some (f6_ref.(regval_of) (f6_ref.(read_from) s))
+  | "f5" => Some (f5_ref.(regval_of) (f5_ref.(read_from) s))
+  | "f4" => Some (f4_ref.(regval_of) (f4_ref.(read_from) s))
+  | "f3" => Some (f3_ref.(regval_of) (f3_ref.(read_from) s))
+  | "f2" => Some (f2_ref.(regval_of) (f2_ref.(read_from) s))
+  | "f1" => Some (f1_ref.(regval_of) (f1_ref.(read_from) s))
+  | "f0" => Some (f0_ref.(regval_of) (f0_ref.(read_from) s))
+  | "float_fflags" => Some (float_fflags_ref.(regval_of) (float_fflags_ref.(read_from) s))
+  | "float_result" => Some (float_result_ref.(regval_of) (float_result_ref.(read_from) s))
+  | "utval" => Some (utval_ref.(regval_of) (utval_ref.(read_from) s))
+  | "ucause" => Some (ucause_ref.(regval_of) (ucause_ref.(read_from) s))
+  | "uepc" => Some (uepc_ref.(regval_of) (uepc_ref.(read_from) s))
+  | "uscratch" => Some (uscratch_ref.(regval_of) (uscratch_ref.(read_from) s))
+  | "utvec" => Some (utvec_ref.(regval_of) (utvec_ref.(read_from) s))
+  | "pmpaddr15" => Some (pmpaddr15_ref.(regval_of) (pmpaddr15_ref.(read_from) s))
+  | "pmpaddr14" => Some (pmpaddr14_ref.(regval_of) (pmpaddr14_ref.(read_from) s))
+  | "pmpaddr13" => Some (pmpaddr13_ref.(regval_of) (pmpaddr13_ref.(read_from) s))
+  | "pmpaddr12" => Some (pmpaddr12_ref.(regval_of) (pmpaddr12_ref.(read_from) s))
+  | "pmpaddr11" => Some (pmpaddr11_ref.(regval_of) (pmpaddr11_ref.(read_from) s))
+  | "pmpaddr10" => Some (pmpaddr10_ref.(regval_of) (pmpaddr10_ref.(read_from) s))
+  | "pmpaddr9" => Some (pmpaddr9_ref.(regval_of) (pmpaddr9_ref.(read_from) s))
+  | "pmpaddr8" => Some (pmpaddr8_ref.(regval_of) (pmpaddr8_ref.(read_from) s))
+  | "pmpaddr7" => Some (pmpaddr7_ref.(regval_of) (pmpaddr7_ref.(read_from) s))
+  | "pmpaddr6" => Some (pmpaddr6_ref.(regval_of) (pmpaddr6_ref.(read_from) s))
+  | "pmpaddr5" => Some (pmpaddr5_ref.(regval_of) (pmpaddr5_ref.(read_from) s))
+  | "pmpaddr4" => Some (pmpaddr4_ref.(regval_of) (pmpaddr4_ref.(read_from) s))
+  | "pmpaddr3" => Some (pmpaddr3_ref.(regval_of) (pmpaddr3_ref.(read_from) s))
+  | "pmpaddr2" => Some (pmpaddr2_ref.(regval_of) (pmpaddr2_ref.(read_from) s))
+  | "pmpaddr1" => Some (pmpaddr1_ref.(regval_of) (pmpaddr1_ref.(read_from) s))
+  | "pmpaddr0" => Some (pmpaddr0_ref.(regval_of) (pmpaddr0_ref.(read_from) s))
+  | "pmp15cfg" => Some (pmp15cfg_ref.(regval_of) (pmp15cfg_ref.(read_from) s))
+  | "pmp14cfg" => Some (pmp14cfg_ref.(regval_of) (pmp14cfg_ref.(read_from) s))
+  | "pmp13cfg" => Some (pmp13cfg_ref.(regval_of) (pmp13cfg_ref.(read_from) s))
+  | "pmp12cfg" => Some (pmp12cfg_ref.(regval_of) (pmp12cfg_ref.(read_from) s))
+  | "pmp11cfg" => Some (pmp11cfg_ref.(regval_of) (pmp11cfg_ref.(read_from) s))
+  | "pmp10cfg" => Some (pmp10cfg_ref.(regval_of) (pmp10cfg_ref.(read_from) s))
+  | "pmp9cfg" => Some (pmp9cfg_ref.(regval_of) (pmp9cfg_ref.(read_from) s))
+  | "pmp8cfg" => Some (pmp8cfg_ref.(regval_of) (pmp8cfg_ref.(read_from) s))
+  | "pmp7cfg" => Some (pmp7cfg_ref.(regval_of) (pmp7cfg_ref.(read_from) s))
+  | "pmp6cfg" => Some (pmp6cfg_ref.(regval_of) (pmp6cfg_ref.(read_from) s))
+  | "pmp5cfg" => Some (pmp5cfg_ref.(regval_of) (pmp5cfg_ref.(read_from) s))
+  | "pmp4cfg" => Some (pmp4cfg_ref.(regval_of) (pmp4cfg_ref.(read_from) s))
+  | "pmp3cfg" => Some (pmp3cfg_ref.(regval_of) (pmp3cfg_ref.(read_from) s))
+  | "pmp2cfg" => Some (pmp2cfg_ref.(regval_of) (pmp2cfg_ref.(read_from) s))
+  | "pmp1cfg" => Some (pmp1cfg_ref.(regval_of) (pmp1cfg_ref.(read_from) s))
+  | "pmp0cfg" => Some (pmp0cfg_ref.(regval_of) (pmp0cfg_ref.(read_from) s))
+  | "tselect" => Some (tselect_ref.(regval_of) (tselect_ref.(read_from) s))
+  | "stval" => Some (stval_ref.(regval_of) (stval_ref.(read_from) s))
+  | "scause" => Some (scause_ref.(regval_of) (scause_ref.(read_from) s))
+  | "sepc" => Some (sepc_ref.(regval_of) (sepc_ref.(read_from) s))
+  | "sscratch" => Some (sscratch_ref.(regval_of) (sscratch_ref.(read_from) s))
+  | "stvec" => Some (stvec_ref.(regval_of) (stvec_ref.(read_from) s))
+  | "sideleg" => Some (sideleg_ref.(regval_of) (sideleg_ref.(read_from) s))
+  | "sedeleg" => Some (sedeleg_ref.(regval_of) (sedeleg_ref.(read_from) s))
+  | "mhartid" => Some (mhartid_ref.(regval_of) (mhartid_ref.(read_from) s))
+  | "marchid" => Some (marchid_ref.(regval_of) (marchid_ref.(read_from) s))
+  | "mimpid" => Some (mimpid_ref.(regval_of) (mimpid_ref.(read_from) s))
+  | "mvendorid" => Some (mvendorid_ref.(regval_of) (mvendorid_ref.(read_from) s))
+  | "minstret_written" => Some (minstret_written_ref.(regval_of) (minstret_written_ref.(read_from) s))
+  | "minstret" => Some (minstret_ref.(regval_of) (minstret_ref.(read_from) s))
+  | "mtime" => Some (mtime_ref.(regval_of) (mtime_ref.(read_from) s))
+  | "mcycle" => Some (mcycle_ref.(regval_of) (mcycle_ref.(read_from) s))
+  | "mcountinhibit" => Some (mcountinhibit_ref.(regval_of) (mcountinhibit_ref.(read_from) s))
+  | "scounteren" => Some (scounteren_ref.(regval_of) (scounteren_ref.(read_from) s))
+  | "mcounteren" => Some (mcounteren_ref.(regval_of) (mcounteren_ref.(read_from) s))
+  | "mscratch" => Some (mscratch_ref.(regval_of) (mscratch_ref.(read_from) s))
+  | "mtval" => Some (mtval_ref.(regval_of) (mtval_ref.(read_from) s))
+  | "mepc" => Some (mepc_ref.(regval_of) (mepc_ref.(read_from) s))
+  | "mcause" => Some (mcause_ref.(regval_of) (mcause_ref.(read_from) s))
+  | "mtvec" => Some (mtvec_ref.(regval_of) (mtvec_ref.(read_from) s))
+  | "medeleg" => Some (medeleg_ref.(regval_of) (medeleg_ref.(read_from) s))
+  | "mideleg" => Some (mideleg_ref.(regval_of) (mideleg_ref.(read_from) s))
+  | "mie" => Some (mie_ref.(regval_of) (mie_ref.(read_from) s))
+  | "mip" => Some (mip_ref.(regval_of) (mip_ref.(read_from) s))
+  | "mstatus" => Some (mstatus_ref.(regval_of) (mstatus_ref.(read_from) s))
+  | "mstatush" => Some (mstatush_ref.(regval_of) (mstatush_ref.(read_from) s))
+  | "misa" => Some (misa_ref.(regval_of) (misa_ref.(read_from) s))
+  | "cur_inst" => Some (cur_inst_ref.(regval_of) (cur_inst_ref.(read_from) s))
+  | "cur_privilege" => Some (cur_privilege_ref.(regval_of) (cur_privilege_ref.(read_from) s))
+  | "x31" => Some (x31_ref.(regval_of) (x31_ref.(read_from) s))
+  | "x30" => Some (x30_ref.(regval_of) (x30_ref.(read_from) s))
+  | "x29" => Some (x29_ref.(regval_of) (x29_ref.(read_from) s))
+  | "x28" => Some (x28_ref.(regval_of) (x28_ref.(read_from) s))
+  | "x27" => Some (x27_ref.(regval_of) (x27_ref.(read_from) s))
+  | "x26" => Some (x26_ref.(regval_of) (x26_ref.(read_from) s))
+  | "x25" => Some (x25_ref.(regval_of) (x25_ref.(read_from) s))
+  | "x24" => Some (x24_ref.(regval_of) (x24_ref.(read_from) s))
+  | "x23" => Some (x23_ref.(regval_of) (x23_ref.(read_from) s))
+  | "x22" => Some (x22_ref.(regval_of) (x22_ref.(read_from) s))
+  | "x21" => Some (x21_ref.(regval_of) (x21_ref.(read_from) s))
+  | "x20" => Some (x20_ref.(regval_of) (x20_ref.(read_from) s))
+  | "x19" => Some (x19_ref.(regval_of) (x19_ref.(read_from) s))
+  | "x18" => Some (x18_ref.(regval_of) (x18_ref.(read_from) s))
+  | "x17" => Some (x17_ref.(regval_of) (x17_ref.(read_from) s))
+  | "x16" => Some (x16_ref.(regval_of) (x16_ref.(read_from) s))
+  | "x15" => Some (x15_ref.(regval_of) (x15_ref.(read_from) s))
+  | "x14" => Some (x14_ref.(regval_of) (x14_ref.(read_from) s))
+  | "x13" => Some (x13_ref.(regval_of) (x13_ref.(read_from) s))
+  | "x12" => Some (x12_ref.(regval_of) (x12_ref.(read_from) s))
+  | "x11" => Some (x11_ref.(regval_of) (x11_ref.(read_from) s))
+  | "x10" => Some (x10_ref.(regval_of) (x10_ref.(read_from) s))
+  | "x9" => Some (x9_ref.(regval_of) (x9_ref.(read_from) s))
+  | "x8" => Some (x8_ref.(regval_of) (x8_ref.(read_from) s))
+  | "x7" => Some (x7_ref.(regval_of) (x7_ref.(read_from) s))
+  | "x6" => Some (x6_ref.(regval_of) (x6_ref.(read_from) s))
+  | "x5" => Some (x5_ref.(regval_of) (x5_ref.(read_from) s))
+  | "x4" => Some (x4_ref.(regval_of) (x4_ref.(read_from) s))
+  | "x3" => Some (x3_ref.(regval_of) (x3_ref.(read_from) s))
+  | "x2" => Some (x2_ref.(regval_of) (x2_ref.(read_from) s))
+  | "x1" => Some (x1_ref.(regval_of) (x1_ref.(read_from) s))
+  | "instbits" => Some (instbits_ref.(regval_of) (instbits_ref.(read_from) s))
+  | "nextPC" => Some (nextPC_ref.(regval_of) (nextPC_ref.(read_from) s))
+  | "PC" => Some (PC_ref.(regval_of) (PC_ref.(read_from) s))
+  | _ => None
+  end.
 
+Lemma get_regval'_eq r regs:
+  get_regval r regs = get_regval' r regs.
+Proof.
+  unfold get_regval.
+  have Hcase : ∀ s e1 e2 (v : option register_value),
+      (r = s → e1 = v) →
+      (r ≠ s → e2 = v) →
+      (if string_dec r s then e1 else e2) = v. {
+    move => s ?????. destruct (string_dec r s); eauto.
+  }
+  repeat (apply Hcase; [move => ->; done| move => ?]).
+  unfold get_regval'.
+  destruct r => //.
+Admitted.
+(*
+  all: destruct r => //. 1: admit.
+  all: destruct r => //.
+  1: destruct a0 as [[] [] [] [] [] [] [] []] => //.
+  all: destruct r => //.
+                    repeat (case_match => //).
+*)
+*)
 Lemma get_set_regval r regs regs' v:
   set_regval r v regs = Some regs' ->
   get_regval r regs' = Some v.
@@ -216,6 +413,20 @@ Lemma get_set_regval_ne r r' regs regs' v:
   r ≠ r' →
   get_regval r regs' = get_regval r regs.
 Proof.
+  (*
+  rewrite !get_regval'_eq.
+  unfold get_regval'.
+  destruct r => //.
+  destruct a as [[] [] [] [] [] [] [] []]; try fast_done.
+  all: destruct r => //.
+  all: destruct a as [[] [] [] [] [] [] [] []]; try fast_done.
+  all: destruct r => //.
+  all: try destruct a as [[] [] [] [] [] [] [] []]; try fast_done.
+
+  destruct (decide (r = String 's' ))
+                    do 100 try case_match => //.
+  - do 100 try case_match => //.
+*)
   unfold set_regval, get_regval.
   move => Hset Hneq.
   have Hcase : ∀ s (e1 e2 e1' e2' : option register_value),
@@ -233,13 +444,48 @@ Proof.
   }
   repeat (apply Hcase; [shelve|]). done.
   Unshelve.
+  (* - clear Hcase. move => ?; subst r. simpl. move: Hset. *)
+  (*   destruct r'. 1: done. *)
+  (*   Set Nested Proofs Allowed. *)
+  (*   Lemma string_dec_length A s1 s2 e1 e2: *)
+  (*     String.length s1 ≠ String.length s2 → *)
+  (*     (if string_dec s1 s2 then e1 else e2) =@{A} e2. *)
+  (*   Proof. Admitted. *)
+  (*   Create HintDb string_dec_rewrite. *)
+  (*   Hint Rewrite string_dec_length using done : string_dec_rewrite. *)
+  (*   destruct r'. 1: { autorewrite with string_dec_rewrite. done. } *)
+  (*   autorewrite with string_dec_rewrite.  *)
+  (*   destruct r'. 1: { autorewrite with string_dec_rewrite. repeat rewrite ->string_dec_length by done. done. } 1: admit. *)
+  (*   destruct r' => //. 1: admit. *)
+  (*   destruct r' => //. 1: admit. *)
+  (*   repeat (apply Hcase2; [shelve|]); done. *)
   (* all: clear Hcase; move => ?; subst r; simpl; move: Hset; repeat (apply Hcase2; [shelve|]); done. *)
 Admitted.
+
+
+Lemma get_regval_None_stable r regs regs':
+  get_regval r regs = None →
+  get_regval r regs' = None.
+Proof.
+  have Hcase : ∀ s (e1 e2 e1' e2' : option register_value),
+      (r = s → e1 = None → e1' = None) →
+      (e2 = None → e2' = None) →
+      (if string_dec r s then e1 else e2) = None →
+      (if string_dec r s then e1' else e2') = None. {
+    move => s ??????. destruct (string_dec r s); eauto.
+  }
+  repeat (apply Hcase; [done|]). done.
+Qed.
+
 
 Lemma getBit_testbit n z (w : Word.word n):
   n ≠ 0%nat →
   getBit w z = Z.testbit (Z.of_N (Word.wordToN w)) (Z.of_nat z).
 Proof. destruct n => //=. Admitted.
+
+Lemma getBit_wordFromBitlist l i:
+  getBit (wordFromBitlist l) i = default false (l !! i).
+Proof. Admitted.
 
 Lemma bit_to_bool_false b:
   b = B0 →
@@ -257,3 +503,153 @@ Lemma bitU_of_bool_B1 b :
   b = true →
   bitU_of_bool b = B1.
 Proof. by move => ->. Qed.
+Lemma access_vec_dec_concrete x n (b : mword n) z:
+  access_vec_dec b z = x →
+  access_vec_dec b z = x.
+Proof. by move => ->. Qed.
+
+Lemma if_true b A (e1 e2 : A):
+  b = true →
+  (if b then e1 else e2) = e1.
+Proof. naive_solver. Qed.
+Lemma if_false b A (e1 e2 : A):
+  b = false →
+  (if b then e1 else e2) = e2.
+Proof. naive_solver. Qed.
+
+
+Lemma option_map_fmap {A B} x (f : A → B):
+  option_map f x = f <$> x.
+Proof. by destruct x. Qed.
+
+Lemma map_fmap {A B} x (f : A → B):
+  map f x = f <$> x.
+Proof. done.  Qed.
+
+Lemma just_list_mapM {A} (l : list (option A)):
+  just_list l = mapM (M := option) id l.
+Proof. elim: l => //= -[|]//= ?? ->. case_match => //. Qed.
+
+Lemma byte_chunks_reshape {A} n (l : list A):
+  (length l = n * 8)%nat →
+  byte_chunks l = Some (reshape (replicate n 8%nat) l).
+Proof.
+  move Hlen: (length l) => len.
+  elim/lt_wf_ind: len l n Hlen => len IH l n ?. subst.
+  destruct l => //=. { by destruct n. }
+  do 7 (destruct l => /=; [lia|]). move => ?.
+  have ?: (length l = ((n-1) * 8))%nat by lia.
+  erewrite IH; [..|done]; [|simpl;lia|done].
+  have {2}-> : (n = S (n-1)) by lia.
+  by rewrite /= take_0 drop_0.
+Qed.
+
+Lemma rev_lookup {A} (l : list A) i:
+  (i < length l)%nat →
+  rev l !! i = l !! (length l - 1 - i)%nat.
+Proof.
+  elim: l i => //= x l IH i ?.
+  destruct (decide (i = length l)); subst.
+  + rewrite list_lookup_middle ?rev_length //.
+    by have ->: (length l - 0 - length l = 0)%nat by lia.
+  + rewrite lookup_app_l ?rev_length; [|lia].
+    rewrite IH; [|lia].
+    by have ->: (length l - 0 - i = S (length l - 1 - i))%nat by lia.
+Qed.
+
+Lemma length_bitlistFromWord_rev n (w : Word.word n):
+  length (bitlistFromWord_rev w) = n.
+Proof.
+  elim: n w. { move => w. have ->:= Word.shatter_word_0 w. done. }
+  move => n IH w. have [b [c ->]]:= Word.shatter_word_S w => /=. by rewrite IH.
+Qed.
+
+Lemma length_bitlistFromWord n (w : Word.word n):
+  length (bitlistFromWord w) = n.
+Proof. by rewrite /bitlistFromWord rev_length length_bitlistFromWord_rev. Qed.
+
+Lemma fit_bbv_word_id n1 n2 (m : Word.word n1):
+  ∀ Heq : n1 = n2, fit_bbv_word m = eq_rect n1 _ m n2 Heq.
+Proof.
+  move => Heq. destruct Heq => /=.
+  rewrite /fit_bbv_word.
+Admitted.
+
+Lemma sum_list_fmap {A} n (l : list A) f:
+  (∀ x, x ∈ l → f x = n) →
+  sum_list (f <$> l) = (length l * n)%nat.
+Proof. move => Hf. elim: l Hf => //; csimpl=> ?? IH Hf. rewrite IH. 2: set_solver. rewrite Hf //. set_solver. Qed.
+
+Lemma sum_list_fmap' {A} (l : list A) n :
+  sum_list ((λ _, n) <$> l) = (length l * n)%nat.
+Proof. by apply sum_list_fmap. Qed.
+
+Lemma concat_join {A} (l : list (list A)):
+  concat l = mjoin l.
+Proof. by elim: l => // ??; csimpl => ->. Qed.
+Lemma rev_reverse {A} (l : list A):
+  rev l = reverse l.
+Proof. elim: l => // ??/= ->. by rewrite reverse_cons. Qed.
+
+Lemma length_bits_of_bytes l:
+  (∀ x, x ∈ l → length x = 8%nat) →
+  length (bits_of_bytes l) = (length l * 8)%nat.
+Proof.
+  move => Hf.
+  rewrite /bits_of_bytes concat_join map_fmap join_length -list_fmap_compose /compose.
+  rewrite (sum_list_fmap 8) // => ?. rewrite /bits_of/= map_fmap fmap_length. apply: Hf.
+Qed.
+
+Lemma length_bits_of_mem_bytes l:
+  (∀ x, x ∈ l → length x = 8%nat) →
+  length (bits_of_mem_bytes l) = (length l * 8)%nat.
+Proof.
+  move => Hf. rewrite length_bits_of_bytes ?rev_length // => ?.
+  rewrite rev_reverse elem_of_reverse. apply: Hf.
+Qed.
+
+Lemma join_lookup_Some {A} (ls : list (list A)) i x:
+  mjoin ls !! i = Some x ↔ ∃ j l i', ls !! j = Some l ∧ l !! i' = Some x
+                             ∧ i = (sum_list (length <$> take j ls) + i')%nat.
+Proof.
+  elim: ls i; csimpl. 1: set_solver.
+  move => ?? IH i. rewrite lookup_app_Some IH.
+  split.
+  - case.
+    + move => ?. by eexists 0%nat, _, _.
+    + move => [? [?[?[?[?[??]]]]]]. eexists (S _), _, _. split_and! => //; csimpl. lia.
+  - move => [j [?[?[?[? ->]]]]]. destruct j as [|j]; csimpl in *.
+    + left. naive_solver.
+    + right. split; [lia|]. eexists _, _, _. split_and! => //. lia.
+Qed.
+
+Lemma join_lookup_Some' {A} n (ls : list (list A)) i x:
+  (∀ x, x ∈ ls → length x = n) →
+  mjoin ls !! i = Some x ↔ ∃ j l i', ls !! j = Some l ∧ l !! i' = Some x
+                             ∧ i = (j * n + i')%nat.
+Proof.
+  move => Hl. rewrite join_lookup_Some.
+Admitted.
+
+Lemma join_lookup_Some_mul {A} n (ls : list (list A)) j i x:
+  (∀ x, x ∈ ls → length x = n) →
+  (i < n)%nat →
+  mjoin ls !! (j * n + i)%nat = Some x ↔ ∃ l, ls !! j = Some l ∧ l !! i = Some x.
+Proof.
+  move => Hf ?. rewrite join_lookup_Some' //. split; [| naive_solver].
+  move => [j'[l'[i'[?[??]]]]].
+  have ? : (i' < n)%nat. { erewrite <-Hf; [| by eapply elem_of_list_lookup_2]. by eapply lookup_lt_Some. }
+  have ?: j = j' by nia. subst. have : i = i' by lia. naive_solver.
+Qed.
+Lemma rev_lookup_Some {A} (l : list A) i x:
+  rev l !! i = Some x ↔ l !! (length l - 1 - i)%nat = Some x ∧ (i < length l)%nat.
+Proof.
+  split.
+  - destruct (decide (i < length l)%nat). 1: by rewrite rev_lookup.
+    rewrite lookup_ge_None_2 // rev_length. lia.
+  - move => [??]. by rewrite rev_lookup.
+Qed.
+
+Lemma bool_of_bitU_of_bool b:
+  bool_of_bitU (bitU_of_bool b) = Some b.
+Proof. by destruct b. Qed.
