sail-riscv/riscv64_test.v
@@ -4,6 +4,7 @@ Require Import Sail.State_lifting.
 Require Import isla.sail_riscv.sail_opsem.
 Require Import isla.sail_riscv.tactics.
 Require Import isla.automation.
+Require Import isla.riscv64.riscv64.
 From isla.instructions.riscv64_test Require Import instrs.
 Require Import isla.examples.riscv64_test.
 
@@ -13,9 +14,8 @@ Proof.
   move => regs. eexists _. split; [by left|].
   unfold step_cpu. red_sim. unfold execute. red_sim.
   unfold execute_ITYPE. red_sim.
-  Unshelve.
-  all: try done.
-  - simpl. destruct regs => /=. rewrite mword_to_bv_add_vec //.
+  Unshelve. all: sim_simpl_goal.
+  - rewrite mword_to_bv_add_vec //.
 Qed.
 
 Lemma sim_instr_a4:
@@ -24,26 +24,106 @@ Proof.
   move => regs. eexists _. split; [by left|].
   unfold step_cpu. red_sim. unfold execute. red_sim.
   unfold execute_ITYPE. red_sim.
-  Unshelve.
-  all: try done.
-  - simpl. destruct regs => /=. rewrite mword_to_bv_add_vec //.
-  - simpl. destruct regs => /=. rewrite mword_to_bv_add_vec //.
+  Unshelve. all: sim_simpl_goal.
+  all: rewrite mword_to_bv_add_vec //.
 Qed.
 
 Lemma sim_instr_a8:
-  sim_instr (Uncompressed [BV{32} 0x00b50463]) a8.
+  sim_instr (Uncompressed [BV{32} 0x00b13423]) a8.
+Proof.
+  move => regs. eexists _. split; [by left|].
+  unfold step_cpu. red_sim. unfold execute. red_sim.
+  unfold execute_STORE. red_sim. rewrite x2_nextPC.
+  unfold check_misaligned. rewrite Hassume0.
+  repeat (rewrite (access_vec_dec_concrete B0); [|shelve]).
+  red_sim.
+  unfold translateAddr. red_sim.
+  unfold effectivePrivilege. red_sim.
+  rewrite mstatus_nextPC.
+  have -> : (_get_Mstatus_MPRV (mstatus regs)) = ('b "0") by shelve.
+  red_sim.
+  unfold translateAddr_priv. red_sim.
+  apply: sim_read_reg_l; [done|]. red_sim.
+  apply: sim_read_reg_l; [done|]. red_sim.
+  unfold translationMode. rewrite cur_privilege_nextPC.
+  have -> : (cur_privilege regs) = Machine by shelve. red_sim.
+  apply: sim_read_reg_l; [done|]. red_sim. rewrite x11_nextPC.
+  unfold mem_write_value, mem_write_value_meta. red_sim.
+  apply: sim_read_reg_l; [done|]. red_sim.
+  apply: sim_read_reg_l; [done|]. red_sim.
+  unfold effectivePrivilege. red_sim. rewrite mstatus_nextPC.
+  have -> : (_get_Mstatus_MPRV (mstatus regs)) = ('b "0") by shelve.
+  red_sim. rewrite Hassume. red_sim.
+  rewrite if_false; [|shelve]. rewrite if_true; [|shelve]. red_sim.
+  Unshelve. all: sim_simpl_goal.
+  all: rewrite -?Hassume1 -?Hassume2 -?Hassume3 -?Hassume4 -?Hassume5 -?Hassume6 -?Hassume7 //.
+  - admit.
+  - admit.
+  - admit.
+  - admit.
+  - admit.
+  - admit.
+  - rewrite Hassume9. by apply bv_neq.
+  - admit.
+  - admit.
+  - rewrite Hassume9. by apply bv_neq.
+  - admit.
+  - admit.
+  - admit.
+  - admit.
+  - admit.
+  - admit.
+  - admit.
+  - admit.
+  - admit.
+  - admit.
+  - admit.
+Admitted.
+
+Lemma sim_instr_ac:
+  sim_instr (Uncompressed [BV{32} 0x00813583]) ac.
+Proof.
+  move => regs. eexists _. split; [by left|].
+  unfold step_cpu. red_sim. unfold execute. red_sim.
+  unfold execute_LOAD. red_sim.
+  unfold check_misaligned. rewrite Hassume0.
+  repeat (rewrite (access_vec_dec_concrete B0); [|shelve]).
+  red_sim.
+  unfold translateAddr. red_sim.
+  unfold effectivePrivilege. red_sim.
+  rewrite mstatus_nextPC.
+  have -> : (_get_Mstatus_MPRV (mstatus regs)) = ('b "0") by shelve.
+  red_sim.
+  unfold translateAddr_priv. red_sim.
+  apply: sim_read_reg_l; [done|]. red_sim.
+  apply: sim_read_reg_l; [done|]. red_sim.
+  unfold translationMode. rewrite cur_privilege_nextPC.
+  have -> : (cur_privilege regs) = Machine by shelve. red_sim.
+  apply: sim_read_reg_l; [done|]. red_sim. rewrite x2_nextPC.
+  unfold mem_read. red_sim.
+  apply: sim_read_reg_l; [done|]. red_sim.
+  apply: sim_read_reg_l; [done|]. red_sim.
+  unfold effectivePrivilege. red_sim. rewrite mstatus_nextPC.
+  have -> : (_get_Mstatus_MPRV (mstatus regs)) = ('b "0") by shelve.
+  red_sim.
+  have -> : plat_enable_pmp () = false by simplify_eq. red_sim.
+  rewrite if_false; [|shelve]. rewrite if_true; [|shelve]. red_sim.
+  Unshelve. all: sim_simpl_goal.
+Admitted.
+
+Lemma sim_instr_a10:
+  sim_instr (Uncompressed [BV{32} 0x00b50463]) a10.
 Proof.
   move => regs.
-  destruct (eq_vec (x10 regs) (x11 regs)) eqn: Hb1.
+  destruct (eq_vec (x10 regs) (x11 regs)) eqn: Hb1; sim_simpl_hyp Hb1.
   all: eexists _; split. 1: by right; left. 2: by left.
   all: unfold step_cpu; red_sim; unfold execute; red_sim.
   all: unfold execute_BTYPE; red_sim.
   all: apply: sim_read_reg_l; [done|]; red_sim.
   all: rewrite x10_nextPC x11_nextPC Hb1; red_sim.
   rewrite bit_to_bool_false; [|shelve]. red_sim.
-  Unshelve.
-  all: rewrite /= ?x10_nextPC ?x11_nextPC ?PC_nextPC ?nextPC_nextPC; simpl; try done.
-  - rewrite (eq_vec_to_bv 64) // in Hb1. by rewrite Hb1.
+  Unshelve. all: sim_simpl_goal.
+  - rewrite (eq_vec_to_bv 64) // bool_decide_eq_true in Hb1. by rewrite Hb1.
   - move: Hassume. normalize_and_simpl_goal => //= Hb.
     have Hbit : (Z.testbit (bv_unsigned (mword_to_bv (n2:=64) (PC regs))) 1) = false. {
       rename select (bv_extract 1 1 _ = _) into He.
@@ -61,7 +141,7 @@ Proof.
     }
     bits_simplify. have ? : n = 0 by lia. subst.
     by rewrite Z.add_bit1 Hbit andb_false_r.
-  - rewrite (eq_vec_to_bv 64) // in Hb1. by rewrite Hb1.
+  - rewrite (eq_vec_to_bv 64) // bool_decide_eq_false in Hb1. done.
   - rewrite mword_to_bv_add_vec //.
   - move: Hassume. normalize_and_simpl_goal => //=.
     apply bitU_of_bool_B0.
@@ -82,38 +162,63 @@ Qed.
 Definition riscv_test_sail_instrs : gmap addr encoded_instruction :=
   <[ [BV{64} 0x0000000010300000] := Uncompressed [BV{32} 0x00000513]]> $
   <[ [BV{64} 0x0000000010300004] := Uncompressed [BV{32} 0x00150513]]> $
-  <[ [BV{64} 0x0000000010300008] := Uncompressed [BV{32} 0x00b50463]]> $
+  <[ [BV{64} 0x0000000010300008] := Uncompressed [BV{32} 0x00b13423]]> $
+  <[ [BV{64} 0x000000001030000c] := Uncompressed [BV{32} 0x00813583]]> $
+  <[ [BV{64} 0x0000000010300010] := Uncompressed [BV{32} 0x00b50463]]> $
   ∅.
 
-Definition riscv_test_initial_sail_state (regs : regstate) : sail_state :=
-  SAIL (Done tt) regs ∅ riscv_test_sail_instrs false.
+Definition riscv_test_initial_sail_state (x2v : bv 64) (regs : regstate) : sail_state :=
+  SAIL (Done tt) regs (riscv_test_state_global x2v).(seq_mem) riscv_test_sail_instrs false.
 
-Lemma riscv_test_safe regs (x11v : bv 64):
+Lemma riscv_test_safe regs (satpv x10v x2v mstatus_bits x11v : bv 64):
+  plat_enable_pmp () = false →
+  plat_enable_misaligned_access () = false →
+  mword_to_bv (plat_ram_base ()) = [BV{64} 0x0000000080000000] →
+  mword_to_bv (plat_ram_size ()) = [BV{64} 0x0000000004000000] →
+  mword_to_bv (plat_rom_base ()) = [BV{64} 0x0000000000001000] →
+  mword_to_bv (plat_rom_size ()) = [BV{64} 0x0000000000000100] →
+  mword_to_bv (plat_clint_base ()) = [BV{64} 0x0000000002000000] →
+  mword_to_bv (plat_clint_size ()) = [BV{64} 0x00000000000c0000] →
+  mword_to_bv (plat_htif_tohost ()) = [BV{64} 0x0000000040001000] →
+  bv_extract 17 1 mstatus_bits = [BV{1} 0] →
+  bv_unsigned x2v `mod` 8 = 0 →
+  0x0000000080000000 ≤ bv_unsigned x2v + 8 < 0x0000000080000000 + 0x0000000004000000 →
   PC regs = bv_to_mword [BV{64} 0x0000000010300000] →
+  x2 regs = bv_to_mword x2v →
+  x10 regs = bv_to_mword x10v →
   x11 regs = bv_to_mword x11v →
+  satp regs = bv_to_mword satpv →
+  cur_privilege regs = Machine →
   misa regs = {| Misa_Misa_chunk_0 := bv_to_mword misa_bits |} →
-  safe sail_module (riscv_test_initial_sail_state regs) ∧
-    (∀ κs σ', steps sail_module (riscv_test_initial_sail_state regs) κs σ' → riscv_test_spec x11v κs).
+  mstatus regs = {| Mstatus_Mstatus_chunk_0 := bv_to_mword mstatus_bits |} →
+  safe sail_module (riscv_test_initial_sail_state x2v regs) ∧
+    (∀ κs σ', steps sail_module (riscv_test_initial_sail_state x2v regs) κs σ' → riscv_test_spec x11v κs).
 Proof.
-  move => HPC Hx11 Hmisa.
+  move => ????????? ??? HPC Hx2 Hx10 Hx11 Hsatp Hcur_priv Hmisa Hmstatus.
   apply: iris_transfer_refines.
   { apply iris_module_wf_isla_lang. }
-  { apply riscv_test_adequate. }
-  apply: sim_implies_refines.
+  { move => ????. by apply (riscv_test_adequate mstatus_bits satpv x2v x10v x11v). }
+  eapply sim_implies_refines.
   - rewrite !dom_insert_L !dom_empty_L. set_solver.
   - move => ??.
     repeat move => /lookup_insert_Some[[??]|[? ]]; simplify_map_eq => //.
-    all: unfold get_regval; simpl; eexists _; split; [done|].
+    all: unfold get_regval_or_config; simpl; eexists _; split; [done|]; sim_simpl_goal.
     + by rewrite HPC.
-    + done.
-    + rewrite Hx11 /= mword_to_bv_to_mword //.
-    + rewrite Hmisa /= mword_to_bv_to_mword //.
+    + by rewrite Hx2 mword_to_bv_to_mword.
+    + by rewrite Hx10 mword_to_bv_to_mword.
+    + by rewrite Hx11 mword_to_bv_to_mword.
+    + by rewrite Hcur_priv.
+    + by rewrite Hmisa.
+    + by rewrite Hmstatus mword_to_bv_to_mword.
+    + by rewrite Hsatp mword_to_bv_to_mword.
   - done.
   - unfold riscv_test_sail_instrs. move => ??? Hsail.
     repeat move => /lookup_insert_Some[[??]|[? ]]; simplify_map_eq.
     + apply sim_instr_a0.
     + apply sim_instr_a4.
     + apply sim_instr_a8.
+    + apply sim_instr_ac.
+    + apply sim_instr_a10.
 Qed.
 
 (* Print Assumptions riscv_test_safe. *)
