sail-riscv/tactics.v
@@ -3,6 +3,8 @@ Require Import Sail.State_monad.
 Require Import Sail.State_lifting.
 Require Import isla.sail_riscv.sail_opsem.
 
+Arguments read_accessor : simpl nomatch.
+
 Ltac hnf_sim :=
   match goal with
   | |- sim _ ?e1 _ _ =>
@@ -17,8 +19,11 @@ Ltac reduce_closed_sim :=
    | |- context [vec_of_bits ?l] => progress reduce_closed (vec_of_bits l)
    | |- context [Word.weqb ?b1 ?b2] => progress reduce_closed (Word.weqb b1 b2)
    | |- context [@eq_vec ?n ?b1 ?b2] => progress reduce_closed (@eq_vec n b1 b2)
+   | |- context [eq_bit ?b1 ?b2] => progress reduce_closed (eq_bit b1 b2)
    (* | |- context [cast_unit_vec ?b] => progress reduce_closed (cast_unit_vec b) *)
    | |- context [@neq_vec ?n ?b1 ?b2] => progress reduce_closed (@neq_vec n b1 b2)
+   | |- context [@generic_eq ?T ?x ?y ?D] => progress reduce_closed (@generic_eq T x y D)
+   | |- context [@generic_neq ?T ?x ?y ?D] => progress reduce_closed (@generic_neq T x y D)
    | |- context [Z.ltb ?n1 ?n2] => progress reduce_closed (Z.ltb n1 n2)
    | |- context [Z.leb ?n1 ?n2] => progress reduce_closed (Z.leb n1 n2)
    | |- context [Z.geb ?n1 ?n2] => progress reduce_closed (Z.geb n1 n2)
@@ -52,24 +57,70 @@ Ltac reduce_closed_sim :=
 
 Ltac cbn_sim :=
   cbn [returnm bind bind0 sim_regs
-       x9_ref x10_ref x11_ref misa_ref PC_ref nextPC_ref
+       x2_ref x9_ref x10_ref x11_ref misa_ref mstatus_ref PC_ref nextPC_ref cur_privilege_ref
        regval_of of_regval read_from write_to regval_from_reg
        Misa_of_regval regval_of_Misa
+       read_kind_of_flags
        ext_control_check_pc
        bitU_of_bool bool_of_bitU bit_to_bool
+       extend_value MemoryOpResult_drop_meta
        negb sumbool_of_bool set
        projT1 build_ex __id andb orb
        _rec_execute compressed_measure Zwf_guarded
        subst_val_event subst_val_valu subst_val_smt subst_val_exp subst_val_base_val fmap list_fmap eq_var_name Z.eqb Pos.eqb map
     ].
 
+Create HintDb simpl_regs_rewrite.
+#[export]
+Hint Rewrite x2_nextPC x10_nextPC nextPC_x10 x11_nextPC nextPC_x11 mstatus_nextPC misa_nextPC
+  cur_privilege_nextPC PC_nextPC nextPC_nextPC : simpl_regs_rewrite.
+Ltac sim_simpl_regs :=
+  autorewrite with simpl_regs_rewrite.
+
+(* Create HintDb mword_to_bv_rewrite. *)
+(* #[export] *)
+(* Hint Rewrite @mword_to_bv_add_vec using done : mword_to_bv_rewrite. *)
+
+Ltac shelve_types :=
+  lazymatch goal with
+  | |- ?G =>
+      lazymatch type of G with
+      | Prop => idtac
+      | _ => shelve
+      end
+  end.
+Ltac sim_simpl_goal :=
+  shelve_types; simpl; sim_simpl_regs;
+  repeat lazymatch goal with
+         | |- Some ?a = Some ?b => apply f_equal_help; [done|]
+         | |- Val_Bool ?a = Val_Bool ?b => apply f_equal_help; [done|]
+         | |- Val_Bits ?a = Val_Bits ?b => apply f_equal_help; [done|]
+         | |- bv_to_bvn ?a = bv_to_bvn ?b => apply f_equal_help; [done|]
+         | |- Val_Enum ?a = Val_Enum ?b => apply f_equal_help; [done|]
+         | |- RegVal_Base ?a = RegVal_Base ?b => apply f_equal_help; [done|]
+         | |- RegVal_Struct ?a = RegVal_Struct ?b => apply f_equal_help; [done|]
+         | |- Mk_enum_id ?a = Mk_enum_id ?b => apply f_equal_help; [done|]
+         | |- (?a1, ?a2) = (?b1, ?b2) => apply f_equal_help; [apply f_equal_help; [done|] |]
+         | |- _::_ = _::_ => apply f_equal_help; [apply f_equal_help; [done|] |]
+         end;
+  try apply negb_true_iff;
+  try apply bool_decide_eq_true_2;
+  try apply bool_decide_eq_false_2;
+  (* autorewrite with mword_to_bv_rewrite; *)
+  try done.
+
 (* Ltac subst_sim := *)
 (*   repeat lazymatch goal with *)
 (*          | H : ?F (sim_regs ?Σ) = _ |- context [?F (sim_regs ?Σ)] => rewrite H *)
 (*          end. *)
+Ltac sim_simpl_hyp H :=
+  try (injection H; clear H; intros H);
+  try apply bool_decide_eq_true_1 in H;
+  try apply bool_decide_eq_false_1 in H;
+  try (apply Eqdep_dec.inj_pair2_eq_dec in H; [|by move => ??; apply decide; apply _]).
 
 Ltac red_monad_sim :=
-  repeat lazymatch goal with
+  repeat match goal with
          | |- sim _ (_ >>= _) _ _  => apply sim_bind
          | |- sim _ (_ >> _) _ _  => apply sim_bind
          | |- sim _ (and_boolM _ _) _ _  => apply sim_bind
@@ -81,21 +132,40 @@ Ltac red_monad_sim :=
          | |- sim _ (Done _) (TryMCtx _ _) _  => apply sim_pop_try_Done
          | |- sim _ (assert_exp' _ _) _ _  => apply sim_assert_exp';
               [try done; shelve| let H := fresh in move => H; try clear H]
-         | |- sim _ _ _ (Smt (DeclareConst _ (Ty_BitVec _)) _::_)  => apply: sim_DeclareConstBitVec
+         | |- sim _ _ _ (Smt (DeclareConst _ Ty_Bool) _::_)  => apply: sim_DeclareConstBool
+         | |- sim _ _ _ (Smt (DeclareConst _ (Ty_BitVec _)) _::?e2) =>
+             lazymatch e2 with
+             | ReadMem _ _ _ _ _ _ :: _ => fail
+             | _ => apply: sim_DeclareConstBitVec
+             end
+         | |- sim _ _ _ (Smt (DeclareConst _ (Ty_Enum _)) _::_)  => apply: sim_DeclareConstEnum
          | |- sim _ _ _ (Smt (DefineConst _ _) _::_)  => apply: sim_DefineConst; [simpl; done|]
          | |- sim _ _ _ (Smt (Assert _) _::_)  => apply: sim_Assert; [simpl; shelve|]
          | |- sim _ _ _ (Branch _ _ _::_)  => apply: sim_Branch
          | |- sim _ _ _ (BranchAddress _ _::_)  => apply: sim_BranchAddress
-         | |- sim _ _ _ (Assume _ _::_)  => let H := fresh "Hassume" in apply: sim_Assume => H; simpl in H
+         | |- sim _ _ _ (Assume _ _::_)  =>
+             let H := fresh "Hassume" in apply: sim_Assume => H; simpl in H; sim_simpl_hyp H
+         | |- sim _ _ _ (AssumeReg _ _ _ _::_)  =>
+             let H := fresh "Hassume" in apply: sim_AssumeReg => H; simpl in H; sim_simpl_hyp H
+         | |- sim _ _ _ (ReadReg _ _ _ _::_)  => apply: sim_ReadReg_config; [reflexivity | try done; shelve|]
          | |- sim _ (read_reg _) _ (ReadReg _ _ _ _::_)  => apply: sim_read_reg; [done | done | try done; shelve|]
          | |- sim _ (write_reg nextPC_ref _) _ _  => apply: sim_write_reg_private; [done..|]
          | |- sim _ (read_reg nextPC_ref) _ _  => apply: sim_read_reg_l; [done..|]
          | |- sim _ (write_reg _ _) _ (WriteReg _ _ _ _::_)  => apply: sim_write_reg; [done | shelve |]
+         | |- sim _ (Write_ea _ _ _ _) _ _  => apply: sim_Write_ea
+         | |- sim _ (Prompt_monad.write_mem _ _ _ _ _) _ (WriteMem _ _ _ _ _ _ _ ::_)  => apply sim_write_mem; [done|done|done|done|shelve|shelve|]
+         | |- sim _ (Prompt_monad.read_mem _ _ _ _) _ (Smt (DeclareConst _ (Ty_BitVec _)) _::ReadMem _ _ _ _ _ _ ::_) =>
+             apply sim_read_mem; [done|done|shelve|] => ?? ->
          | |- sim _ (Done _) NilMCtx []  => apply: sim_done
          end.
 
+
 Ltac unfold_sim :=
-  unfold wX_bits, rX_bits, rX, wX, set_next_pc, regval_from_reg, regval_into_reg, returnm, set.
+  unfold wX_bits, rX_bits, rX, wX, set_next_pc, regval_from_reg, regval_into_reg, returnm, set, ext_data_get_addr,
+    mem_write_ea, write_ram_ea, write_mem_ea, phys_mem_write, write_ram, phys_mem_read, read_ram, process_load,
+    mem_write_value_priv_meta, pmp_mem_write, checked_mem_write, mem_read_priv, mem_read_priv_meta, pmp_mem_read,
+    checked_mem_read.
+
 
 Ltac red_sim :=
     repeat first [
